redefine identity monad

cava/Cava/Acorn/Identity.v
@@ -17,35 +17,37 @@
 Require Import Coq.Vectors.Vector.
 Require Import ExtLib.Data.List.
 Require Import ExtLib.Data.Vector.
-Require Import ExtLib.Data.Monads.IdentityMonad.
 Require Import ExtLib.Structures.Monad.
 Require Import ExtLib.Structures.MonadLaws.
 Require Import ExtLib.Structures.Traversable.
 Require Import Cava.VectorUtils.
 
+(* Identity monad *)
+Definition ident (T : Type) := T.
+Instance Monad_ident : Monad ident :=
+  { ret := fun _ t => t;
+    bind := fun _ _ x f => f x }.
+
+Instance MonadLaws_ident : MonadLaws Monad_ident.
+Proof. econstructor; intros; exact eq_refl. Defined.
+
 Section MapT.
   Lemma mapT_vector_ident {A B n} (f : A -> ident B) (v : Vector.t A n) :
-    unIdent (mapT_vector f v) = Vector.map (fun a => unIdent (f a)) v.
+    mapT_vector f v = Vector.map f v.
   Proof.
     induction v; intros; [ reflexivity | ].
     cbn. rewrite IHv. reflexivity.
   Qed.
+
   (* Alternate form of the above with the Traversable wrapper not simplified *)
   Lemma mapT_vident {A B n} (f : A -> ident B) (v : Vector.t A n) :
-    unIdent (Traversable.mapT
-               (Traversable:=Traversable_vector)
-               f v) = Vector.map (fun a => unIdent (f a)) v.
+    mapT (Traversable:=Traversable_vector) f v = Vector.map f v.
   Proof. apply mapT_vector_ident. Qed.
 
   Lemma mapT_lident {A B} (f : A -> ident B) (l : list A) :
-    unIdent (Traversable.mapT
-               (Traversable:=Traversable_list)
-               f l) = List.map (fun a => unIdent (f a)) l.
+    mapT (Traversable:=Traversable_list) f l = List.map f l.
   Proof.
     simpl. induction l; [ reflexivity | ].
     simpl. rewrite IHl. reflexivity.
   Qed.
 End MapT.
-
-Instance MonadLaws_ident : MonadLaws Monad_ident.
-Proof. econstructor; intros; exact eq_refl. Defined.
